# Exercise: Introduction
## Exercise 1.
Give another possible calculation for the result of `double (double 2)`

```haskell
double x = x+x
double (double 2)   -- 8
double (2 + 2)      -- 8
double 4            -- 8
double 2 + double 2 -- 8
double 2 + 4        -- 8
doubledouble x = 4*x
doubledouble 2      -- 8
```

## Exercise 2.
Show that `sum [x] = x` for any number x.

```haskell
sum [] = 0
sum (n:ns) = n + sum ns
sum []
```

â†’ Given exactly ONE number, sum is this number plus the base case (0).

eg.
```haskell
sum [k]
-- = {applying sum}
--   k + (sum [])
-- = {applying sum}
--   k + 0
-- = {applying +}
--   k
```

```haskell
isTrue k = sum [k] == k
allTrue [] = True
allTrue (n:ns) = (&&) (isTrue n) (allTrue ns)
```

## Exercise 3
Define a function `product` that produces the product of a list of numbers, and show using your definition that `product [2,3,4] = 24`

```haskell
product [n] = n
product (n:ns) = n * product ns
product [2,3,4]
-- = {applying product}
--   2 * product [3, 4]
-- = {applying product}
--   2 * (3 * product [4])
-- = {applying product}
--   2 * (3 * 4)
-- = {applying * }
--   24
```

## Exercise 4
How  should  the  definition  of  the  function `qsort` be  modified that it produces a reverse sorted version of a list?

```haskell
qsort [] = []
qsort (x:xs) = qsort smaller ++ [x] ++ qsort larger
                where
                    smaller = [a | a <- xs, a <=x ]
                    larger = [b | b <- xs, b > x]
```


```haskell
rqsort [] = []
rqsort (x:xs) = rqsort larger ++ [x] ++ rqsort smaller
                where
                    smaller = [a | a <- xs, a <=x ]
                    larger = [b | b <- xs, b > x]
```

## Exercise 5
What would be the effect of replacing `<=` by `<` in the original denition of `qsort`? Hint:  consider the example `qsort [2,2,3,1,1]`.

Equal values will be overridden. The sort algorithm builds a new list with all smaller values  + the current value + all larger values. If in the smaller version `<` is used, the recursion for equal values is only called once.

!!! note

    * `++` appends two lists
    * `smaller = [a | a <- xs, a <=x ]` is similar to list comprehensions in Python

!!! warning

    http://stackoverflow.com/questions/26054046/haskell-non-exhaustive-patterns

# Exercise:  First Steps
## Exercise 1
Work through the examples of chapter "First Steps" using GHC

```haskell
double x = x + x
quadruple x = double (double x)
factorial n = product [1..n]

average ns = sum ns `div` length ns

-- This...
a = b + c
    where
        b = 1
        c = 2
d = a * 2
-- ... is equivalent to
-- a = b + c where {b = 1; c = 2}; d = a*2

{- This is

a


multiline
comment-}

-- this is a single line comment
```

## Exercise 2
Parenthesise the following numeric expressions:

```haskell
2^3*4    -- (2^3)*4
2*3+4*5  -- (2*3)+(4*5)
2+3*4^5  -- 2+(3*(4^5))
```

## Exercise 3
The script below contains three syntactic errors.  Correct these errors and
then check that your script works properly using GHCi.

```haskell
N = a 'div' length xs
    where
        a = 10
        xs = [1,2,3,4,5]
```

```haskell
n = a `div` length xs
    where
        a = 10
        xs = [1,2,3,4,5]
```

(`div` integer division truncated toward negative infinity)

## Exercise 4
The library function `last` selects the last element of a non-empty list;  for example, last [1,2,3,4,5] = 5. Show how the function `last` could  be defined in terms of the other library functions introduced in chapter "First Steps". Can you think of another possible definition?

```haskell
last xs = head (reverse xs)
last xs = xs !! (length xs - 1)
```

## Exercise 5
The library function `init` removes the last element from a non-empty list; for example, `init [1,2,3,4,5] = [1,2,3,4]`. Show how `init` could similarly be defined in two different ways.

```haskell
init xs = take (length xs - 1) xs
init xs = reverse (tail (reverse xs))
```
